$$
\begin{cases}
m \left[ \dot{u} - vr + wq - x_G (q^2 + r^2) + y_G (pq - \dot{r}) + z_G (pr + \dot{q}) \right] = X_\Sigma \\
m \left[ \dot{v} - wp + ur - y_G (r^2 + p^2) + z_G (qr - \dot{p}) + x_G (qp + \dot{r}) \right] = Y_\Sigma \\
m \left[ \dot{w} - uq + vp - z_G (p^2 + q^2) + x_G (rp - \dot{q}) + y_G (rq + \dot{p}) \right] = Z_\Sigma \\
I_{xx} \dot{p} + I_{yz} \dot{q} + I_{zx} \dot{r} + (I_{xy} p + I_{yy} q + I_{yz} r) p - (I_{xx} p + I_{xy} q + I_{zx} r) q + m \left[ x_G (\dot{v} + vp - up) - y_G (\dot{u} + ur - wp) \right] = N_\Sigma \\
I_{xx} \dot{p} + I_{xy} \dot{q} + I_{zx} \dot{r} + (I_{xx} p + I_{yz} q + I_{zx} r) q - (I_{xy} p + I_{yy} q + I_{yz} r) r + m \left[ y_G (\dot{w} + vp - up) - z_G (\dot{v} + ur - wp) \right] = K_\Sigma \\
I_{xy} \dot{p} + I_{yy} \dot{q} + I_{yz} \dot{r} + (I_{xx} p + I_{xy} q + I_{zx} r) r - (I_{xy} p + I_{yz} q + I_{zz} r) p + m \left[ z_G (\dot{u} + vp - up) - x_G (\dot{w} + ur - wp) \right] = M_\Sigma \\
\dot{x}_0 = u \cos \psi \cos \theta + v (\cos \psi \sin \theta \sin \varphi - \sin \psi \cos \varphi) + w (\cos \psi \sin \theta \cos \varphi + \sin \psi \sin \varphi) \\
\dot{y}_0 = u \sin \psi \cos \theta + v (\sin \psi \sin \theta \sin \varphi + \cos \psi \cos \varphi) + w (\sin \psi \sin \theta \cos \varphi - \cos \psi \sin \varphi) \\
\dot{z}_0 = -u \sin \theta + v \cos \theta \sin \varphi + w \cos \theta \cos \varphi \\
\dot{\varphi}_0 = p + q \tan \theta \sin \varphi + r \tan \theta \cos \varphi \\
\dot{\theta}_0 = q \cos \varphi - r \sin \varphi \\
\dot{\psi}_0 = q \sin \varphi / \cos \theta + r \cos \varphi / \cos \theta
\end{cases}
$$

$$
\begin{align*}
\dot{x}_0 &= u \cos \psi \cos \theta + v (\cos \psi \sin \theta \sin \varphi - \sin \psi \cos \varphi) + w (\cos \psi \sin \theta \cos \varphi + \sin \psi \sin \varphi) \\
\dot{y}_0 &= u \sin \psi \cos \theta + v (\sin \psi \sin \theta \sin \varphi + \cos \psi \cos \varphi) + w (\sin \psi \sin \theta \cos \varphi - \cos \psi \sin \varphi) \\
\dot{z}_0 &= -u \sin \theta + v \cos \theta \sin \varphi + w \cos \theta \cos \varphi \\
\dot{\varphi}_0 &= p + q \tan \theta \sin \varphi + r \tan \theta \cos \varphi \\
\dot{\theta}_0 &= q \cos \varphi - r \sin \varphi \\
\dot{\psi}_0 &= q \sin \varphi / \cos \theta + r \cos \varphi / \cos \theta
\end{align*}
$$

